CertiGC/GCGraph.v
@@ -95,6 +95,7 @@ Lemma MSS_max_unsigned_range: forall n,
 Proof.
   intros. cbv [Archi.ptr64]. destruct H.
   split; auto.
+  assert (n <= MAX_SPACE_SIZE); try lia.
   transitivity MAX_SPACE_SIZE. 1: assumption.
   intro Hx; inv Hx.
 Qed.
@@ -109,16 +110,17 @@ Proof.
 Qed.
 
 Lemma MSS_max_wordsize_signed_range: forall n,
-    0 <= n < MAX_SPACE_SIZE -> Ptrofs.min_signed <= WORD_SIZE * n <= Ptrofs.max_signed.
+    0 <= n <= MAX_SPACE_SIZE -> Ptrofs.min_signed <= WORD_SIZE * n < Ptrofs.max_signed.
 Proof.
   intros. destruct H. split.
   - unfold WORD_SIZE. transitivity 0. 2: lia. rewrite Z.le_lteq. left.
     apply Ptrofs.min_signed_neg.
-  - 
-  rewrite Z.lt_le_pred in H0. rewrite Z.le_lteq. left.
-  apply Z.le_lt_trans with (WORD_SIZE * Z.pred MAX_SPACE_SIZE).
-  unfold WORD_SIZE. 1: lia.
-  unfold MAX_SPACE_SIZE. rewrite Z.mul_pred_r.
+  -
+  (* rewrite Z.lt_le_pred in H0. rewrite Z.le_lteq. left.*)
+  apply Z.le_lt_trans with (WORD_SIZE * MAX_SPACE_SIZE).
+  apply Z.mul_le_mono_nonneg_l. compute; congruence.  auto.
+  unfold WORD_SIZE.
+  unfold MAX_SPACE_SIZE.
   unfold Ptrofs.max_signed, Ptrofs.half_modulus, Ptrofs.modulus, Ptrofs.wordsize,
   Wordsize_Ptrofs.wordsize.
   destruct Archi.ptr64 eqn:?; first [now inversion Heqb | simpl; lia].
@@ -257,19 +259,19 @@ Record space: Type :=
     total_space: Z;
     space_sh: share;
     space_order: 0 <= used_space <= total_space;
-    space_upper_bound: total_space < MAX_SPACE_SIZE;
+    space_upper_bound: total_space <= MAX_SPACE_SIZE;
   }.
 
 Definition null_space: space.
 Proof.
   refine (Build_space nullval 0 0 emptyshare _ _).
   - split; apply Z.le_refl.
-  - unfold MAX_SPACE_SIZE. vm_compute; reflexivity.
+  - unfold MAX_SPACE_SIZE.  apply Z.shiftl_nonneg. lia.
 Defined.
 
 #[export] Instance space_inhabitant: Inhabitant space := null_space.
 
-Lemma total_space_tight_range: forall sp, 0 <= total_space sp < MAX_SPACE_SIZE.
+Lemma total_space_tight_range: forall sp, 0 <= total_space sp <= MAX_SPACE_SIZE.
 Proof.
   intros. split.
   - destruct (space_order sp). transitivity (used_space sp); assumption.
@@ -282,20 +284,20 @@ Proof. intros. apply MSS_max_unsigned_range.
 Qed.
 
 Lemma total_space_signed_range: forall sp,
-    Ptrofs.min_signed <= WORD_SIZE * total_space sp <= Ptrofs.max_signed.
-Proof. intros. apply MSS_max_wordsize_signed_range, total_space_tight_range. Qed.
+    Ptrofs.min_signed <= WORD_SIZE * total_space sp < Ptrofs.max_signed.
+Proof. intros. apply MSS_max_wordsize_signed_range. apply total_space_tight_range. Qed.
 
 Lemma used_space_signed_range: forall sp,
-    Ptrofs.min_signed <= WORD_SIZE * used_space sp <= Ptrofs.max_signed.
+    Ptrofs.min_signed <= WORD_SIZE * used_space sp < Ptrofs.max_signed.
 Proof.
   intros. apply MSS_max_wordsize_signed_range. destruct (space_order sp). split.
-  1: assumption. apply Z.le_lt_trans with (total_space sp). 1: assumption.
+  1: assumption. apply Z.le_trans with (total_space sp). 1: assumption.
   apply (proj2 (total_space_tight_range sp)).
 Qed.
 
 Lemma rest_space_signed_range: forall sp,
     Ptrofs.min_signed <=
-    WORD_SIZE * total_space sp - WORD_SIZE * used_space sp <=
+    WORD_SIZE * total_space sp - WORD_SIZE * used_space sp <
     Ptrofs.max_signed.
 Proof.
   intros. rewrite <- Z.mul_sub_distr_l. apply MSS_max_wordsize_signed_range.
@@ -4525,6 +4527,7 @@ Proof.
      change m with (k + (m-k))
   end.
   rewrite two_p_is_exp by lia.
+  simpl Z.sub.
   apply Z.mul_le_mono_pos_l. reflexivity.
   apply two_p_monotone. simpl. lia. 
 Qed.
